binary_tree.v
@@ -1,0 +1,113 @@
+(**
+  This module defines the binary tree data type, which is used to
+  represent binary trees.
+
+  This library uses binary trees to represent syntax trees.
+
+  Copyright (C) 2018 Larry D. Lee Jr. <llee454@gmail.com>
+
+  This program is free software: you can redistribute it and/or modify
+  it under the terms of the GNU Lesser General Public License as
+  published by the Free Software Foundation, either version 3 of the
+  License, or (at your option) any later version.
+
+  This program is distributed in the hope that it will be useful,
+  but WITHOUT ANY WARRANTY; without even the implied warranty of
+  MERCHANTABILITY or FITNESS FOR A PARTICULAR PURPOSE.  See the
+  GNU Lesser General Public License for more details.
+
+  You should have received a copy of the GNU Lesser General Public
+  License along with this program. If not, see
+  <https://www.gnu.org/licenses/>.
+*)
+Require Import Bool.
+
+Module Binary_Tree.
+
+Section binary_tree.
+
+(** Represents the values stored in binary trees. *)
+Variable Term : Set.
+
+(**
+  Represents binary trees.
+
+  Binary trees can be used to represent
+  many different types of algebraic
+  expressions. Importantly, when flattened,
+  they are isomorphic with lists. Flattening,
+  projecting onto lists, sorting, and folding
+  may be used normalize ("simplify") algebraic
+  expressions.
+*)
+Inductive BTree : Set
+  := leaf : Term -> BTree
+  |  node : BTree -> BTree -> BTree.
+
+(**
+  Accepts a binary tree and returns true iff
+  the tree is a node term.
+*)
+Definition BTree_is_node
+  :  BTree -> bool
+  := BTree_rec
+       (fun _ => bool)
+       (fun _ => false)
+       (fun _ _ _ _ => true).
+
+(**
+  Accepts a binary tree and returns true iff
+  the tree is a leaf term.
+*)
+Definition BTree_is_leaf
+  :  BTree -> bool
+  := BTree_rec
+       (fun _ => bool)
+       (fun _ => true)
+       (fun _ _ _ _ => false).
+
+(**
+  Accepts a binary tree and returns true
+  iff the tree is right associative.
+
+  Note: right associative trees are isomorphic
+  to lists.
+*)
+Definition BTree_is_rassoc
+  :  BTree -> bool
+  := BTree_rec
+       (fun _ => bool)
+       (fun _ => true)
+       (fun t _ _ f
+         => BTree_is_leaf t && f).
+
+(**
+  Proves that the right subtree in a right
+  associative binary tree is also right
+  associative.
+*)
+Theorem BTree_rassoc_thm
+  :  forall t u : BTree, BTree_is_rassoc (node t u) = true -> BTree_is_rassoc u = true.
+Proof
+  fun t u H
+    => proj2 (
+            andb_prop 
+              (BTree_is_leaf t)
+              (BTree_is_rassoc u)
+              H).
+
+End binary_tree.
+
+Arguments leaf {Term} x.
+
+Arguments node {Term} t u.
+
+Arguments BTree_is_leaf {Term} t.
+
+Arguments BTree_is_node {Term} t.
+
+Arguments BTree_is_rassoc {Term} t.
+
+Arguments BTree_rassoc_thm {Term} t u H.
+
+End Binary_Tree.
